generate according to distribution

src/main.lean
@@ -4,15 +4,14 @@ open io
 
 /-! # Uniform generation -/
 
-def random_fin (n : ℕ) : io (fin n.succ) := 
-io.run_rand (rand.random $ fin n.succ)
+def random_num (n : ℕ) : io ℕ := 
+io.rand 1 n
 
--- Given some seed, we generate a random number in `fin n.succ = {0, ..., n}`.
-#eval random_fin 37 >>= print
+-- Given some seed, we generate a random number in `{1, ..., n}`.
+#eval random_num 37 >>= print
 
--- Generate a list of random numbers in `fin n.succ` of size `m`.
-def random_fin_list (n : ℕ) (m : ℕ) : list (io $ fin n.succ) :=
-list.map (λ _, random_fin n) (list.range m) 
+def random_num_list' (n : ℕ) (m : ℕ) : list (io ℕ) :=
+list.map (λ _, random_num n) (list.range m) 
 
 def print_list_io {α : Type*} [has_to_string α] : list (io α) → io (list α)
 | [] := return []
@@ -21,7 +20,59 @@ def print_list_io {α : Type*} [has_to_string α] : list (io α) → io (list α
   xs' ← print_list_io xs,
   return (x' :: xs')
 
-#eval print_list_io (random_fin_list 37 100) >>= print
+-- Generate a list of random numbers uniformly in `{1, ..., n}` of size `m`.
+def random_num_list (n : ℕ) (m : ℕ) : io (list ℕ) :=
+print_list_io $ random_num_list' n m
+
+#eval random_num_list 37 100 >>= print
 
 /-! # Generation given some distribution -/
+
+def normalize_distrib' : list ℕ → list ℕ 
+| [] := []
+| (x :: xs) := (list.sum (x :: xs)) :: normalize_distrib' xs
+
+def normalize_distrib : list ℕ → list ℕ :=
+list.reverse ∘ normalize_distrib' ∘ list.reverse
+
+def list.mono (l : list ℕ) : Prop :=
+∀ (n : ℕ) (hn : n.succ < l.length), l.nth_le n (n.lt_succ_self.trans hn) ≤ l.nth_le n.succ hn
+
+lemma normalize_distrib_mono {l : list ℕ} : list.mono (normalize_distrib l) :=
+sorry
+
+@[derive [decidable_pred]]
+def list.placed (l : list ℕ) (n : ℕ) (i : ℕ) : Prop :=
+if hi : i < l.length then n ≤ l.nth_le i hi else false
+
+lemma lt_length_of_placed {l : list ℕ} {n : ℕ} {i : ℕ} (h : l.placed n i) : 
+  i < l.length :=
+begin
+  rw [list.placed] at h,
+  split_ifs at h with hi hi,
+  exacts [hi, false.elim h],
+end
+
+lemma exists_placed_iff {l : list ℕ} {n : ℕ} : 
+  (∃ i, l.placed n i) ↔ (∃ i, i < l.length ∧ l.placed n i) :=
+⟨λ ⟨i, h⟩, ⟨i, lt_length_of_placed h, h⟩, λ ⟨i, _, h⟩, ⟨i, h⟩⟩
+
+instance {l : list ℕ} {n : ℕ} : decidable (∃ i, l.placed n i) :=
+decidable_of_iff' _ exists_placed_iff
+
+def list.place (l : list ℕ) (hmono : l.mono) (n : ℕ) : ℕ :=
+if hi : ∃ i, l.placed n i then @nat.find (l.placed n) infer_instance hi else l.length
+
+def list.distribute (distrib : list ℕ) (hmono : distrib.mono) : 
+  list ℕ → list ℕ
+| [] := []
+| (x :: xs) := distrib.place hmono x :: list.distribute xs
+
+def random_num_list_distrib (m : ℕ) (distrib : list ℕ) : io (list ℕ) := do 
+  rnd ← random_num_list (list.sum distrib) m,
+  return ((normalize_distrib distrib).distribute normalize_distrib_mono rnd)
+  
+#eval random_num_list_distrib 100 [0, 0, 8, 9, 8, 9] >>= print
+
+
 
